spec/spec/02-actions/02-timeouts.lean
@@ -1,11 +1,10 @@
-import «02-actions».«00-resume»
 import «02-actions».«P-02-promise.create»
 
 open ServerModel
 
 namespace Timeouts
 
-def onPromiseTimeout (id : String) (now : Nat) : M Unit := do
+def onPromiseTimeout (id : String) (_now : Nat) : M Unit := do
   match ← getPromise id with
   | none =>
       pure ()
@@ -15,23 +14,19 @@ def onPromiseTimeout (id : String) (now : Nat) : M Unit := do
       else
         let listeners := p.listeners
         let callbacks := p.callbacks
-        let p :=
-          if p.isTimer then
-            { p with state := .resolved, settledAt := some p.timeoutAt, callbacks := [], listeners := [] }
-          else
-            { p with state := .rejectedTimedout, settledAt := some p.timeoutAt, callbacks := [], listeners := [] }
+        let p := { p.project p.timeoutAt with callbacks := [], listeners := [] }
         setPromise p
         delPromiseTimeout p.id
         match ← getTask p.id with
         | some t =>
-            setTask { t with state := .fulfilled, pid := none, ttl := none }
+            setTask { t with state := .fulfilled, pid := none, ttl := none, resumes := [] }
             delTaskTimeout t.id
         | none =>
             pure ()
         for address in listeners do
           setMessage address (.unblock p.toRecord)
         for awaiterId in callbacks do
-          enqueueResume p.id awaiterId now
+          defer { awaited := p.id, awaiter := awaiterId }
 
 def onTaskRetryTimeout (id : String) (now : Nat) : M Unit := do
   let retryTimeout := (← get).config.retryTimeout
@@ -39,7 +34,8 @@ def onTaskRetryTimeout (id : String) (now : Nat) : M Unit := do
   | none =>
       pure ()
   | some t =>
-      if t.state != .pending then pure ()
+      if t.state != .pending then
+        pure ()
       else
         delTaskTimeout t.id
         setTaskTimeout t.id 0 (now + retryTimeout)
@@ -55,7 +51,8 @@ def onTaskLeaseTimeout (id : String) (now : Nat) : M Unit := do
   | none =>
       pure ()
   | some t =>
-      if t.state != .acquired then pure ()
+      if t.state != .acquired then
+        pure ()
       else
         let t := { t with state := .pending, pid := none, ttl := none }
         setTask t
