spec/spec/02-actions/P-03-promise.settle.lean
@@ -1,36 +1,30 @@
-import «02-actions».«00-resume»
+import «01-objects».«state»
 
 open ServerModel
 
 def promiseSettle (req : PromiseSettleReq) (now : Nat) : M PromiseSettleRes := do
+  if !req.state.settable then
+    return { status := 400 }
   match ← getPromise req.id with
   | none =>
       return { status := 404 }
   | some p =>
-      if p.state == .pending then
-        if p.timeoutAt > now then
-          let listeners := p.listeners
-          let callbacks := p.callbacks
-          let p := { p with state := req.state, value := req.value, settledAt := some now, callbacks := [], listeners := [] }
-          setPromise p
-          delPromiseTimeout p.id
-          match ← getTask p.id with
-          | some t =>
-              setTask { t with state := .fulfilled, pid := none, ttl := none }
-              delTaskTimeout t.id
-          | none =>
-              pure ()
-          for address in listeners do
-            setMessage address (.unblock p.toRecord)
-          for awaiterId in callbacks do
-            enqueueResume p.id awaiterId now
-          return { status := 200, promise := some p.toRecord }
-        else
-          let projected :=
-            if p.isTimer then
-              { p with state := .resolved, settledAt := some p.timeoutAt }
-            else
-              { p with state := .rejectedTimedout, settledAt := some p.timeoutAt }
-          return { status := 200, promise := some projected.toRecord }
-      else
+      if p.state == .pending ∧ p.timeoutAt > now then
+        let listeners := p.listeners
+        let callbacks := p.callbacks
+        let p := { p with state := req.state, value := req.value, settledAt := some now, callbacks := [], listeners := [] }
+        setPromise p
+        delPromiseTimeout p.id
+        match ← getTask p.id with
+        | some t =>
+            setTask { t with state := .fulfilled, pid := none, ttl := none, resumes := [] }
+            delTaskTimeout t.id
+        | none =>
+            pure ()
+        for address in listeners do
+          setMessage address (.unblock p.toRecord)
+        for awaiterId in callbacks do
+          defer { awaited := p.id, awaiter := awaiterId }
         return { status := 200, promise := some p.toRecord }
+      else
+        return { status := 200, promise := some (p.project now).toRecord }
