spec/spec/02-actions/P-04-promise.register_callback.lean
@@ -3,6 +3,8 @@ import «01-objects».«state»
 open ServerModel
 
 def promiseRegisterCallback (req : PromiseRegisterCallbackReq) (now : Nat) : M PromiseRegisterCallbackRes := do
+  if req.awaited == req.awaiter then
+    return { status := 400 }
   match ← getPromise req.awaited with
   | none =>
       return { status := 404 }
@@ -11,18 +13,13 @@ def promiseRegisterCallback (req : PromiseRegisterCallbackReq) (now : Nat) : M P
   | none =>
       return { status := 422 }
   | some pAwaiter =>
-      if !(pAwaiter.tags.has "resonate:target") then return { status := 422 }
-      if pAwaited.state == .pending then
-        if pAwaited.timeoutAt > now then
-          if pAwaiter.state == .pending ∧ pAwaiter.timeoutAt > now then
-            setPromise (pAwaited.addCallback req.awaiter)
-          return { status := 200, promise := some pAwaited.toRecord }
-        else
-          let projected :=
-            if pAwaited.isTimer then
-              { pAwaited with state := .resolved, settledAt := some pAwaited.timeoutAt }
-            else
-              { pAwaited with state := .rejectedTimedout, settledAt := some pAwaited.timeoutAt }
-          return { status := 200, promise := some projected.toRecord }
-      else
+      if !(pAwaiter.tags.has "resonate:target") then
+        return { status := 422 }
+      if !pAwaited.external then
+        return { status := 422 }
+      if pAwaited.state == .pending ∧ pAwaited.timeoutAt > now then
+        if pAwaiter.state == .pending ∧ pAwaiter.timeoutAt > now then
+          setPromise (pAwaited.addCallback req.awaiter)
         return { status := 200, promise := some pAwaited.toRecord }
+      else
+        return { status := 200, promise := some (pAwaited.project now).toRecord }
