spec/spec/02-actions/T-07-task.fulfill.lean
@@ -1,8 +1,10 @@
-import «02-actions».«00-resume»
+import «01-objects».«state»
 
 open ServerModel
 
 def taskFulfill (req : TaskFulfillReq) (now : Nat) : M TaskFulfillRes := do
+  if !req.action.state.settable then
+    return { status := 400 }
   match ← getTask req.id with
   | none =>
       return { status := 404 }
@@ -11,18 +13,21 @@ def taskFulfill (req : TaskFulfillReq) (now : Nat) : M TaskFulfillRes := do
   | none =>
       return { status := 409 }
   | some p =>
-      if t.state != .acquired then return { status := 409 }
-      if p.state != .pending ∨ p.timeoutAt ≤ now then return { status := 409 }
-      if t.version != req.version then return { status := 409 }
+      if t.state != .acquired then
+        return { status := 409 }
+      if p.state != .pending ∨ p.timeoutAt ≤ now then
+        return { status := 409 }
+      if t.version != req.version then
+        return { status := 409 }
       let listeners := p.listeners
       let callbacks := p.callbacks
       let p := { p with state := req.action.state, value := req.action.value, settledAt := some now, callbacks := [], listeners := [] }
       setPromise p
       delPromiseTimeout p.id
-      setTask { t with state := .fulfilled, pid := none, ttl := none }
+      setTask { t with state := .fulfilled, pid := none, ttl := none, resumes := [] }
       delTaskTimeout t.id
       for address in listeners do
         setMessage address (.unblock p.toRecord)
       for awaiterId in callbacks do
-        enqueueResume p.id awaiterId now
+        defer { awaited := p.id, awaiter := awaiterId }
       return { status := 200, promise := some p.toRecord }
